split the files
  - Iteration.thy contains the big proof of the iteration combinator

  - Recursion.thy derives from Iteration the recursion combinator

  - lam_substs.thy contains the examples (size, substitution and parallel substitution)

src/HOL/Nominal/Examples/Lam_substs.thy
@@ -1,1118 +1,9 @@
 (* $Id$ *)
 
 theory lam_substs
-imports "../nominal" 
+imports "Iteration" 
 begin
 
-text {* Contains all the reasoning infrastructure for the
-        lambda-calculus that the nominal datatype package
-        does not yet provide. *}
-
-atom_decl name 
-
-nominal_datatype lam = Var "name"
-                     | App "lam" "lam"
-                     | Lam "\<guillemotleft>name\<guillemotright>lam" ("Lam [_]._" [100,100] 100)
-
-types 'a f1_ty  = "name\<Rightarrow>('a::pt_name)"
-      'a f2_ty  = "'a\<Rightarrow>'a\<Rightarrow>('a::pt_name)"
-      'a f3_ty  = "name\<Rightarrow>'a\<Rightarrow>('a::pt_name)"
-
-lemma f3_freshness_conditions:
-  fixes f3::"('a::pt_name) f3_ty"
-  and   y ::"name prm \<Rightarrow> 'a::pt_name"
-  and   a ::"name"
-  and   pi1::"name prm"
-  and   pi2::"name prm"
-  assumes a: "finite ((supp f3)::name set)"
-  and     b: "finite ((supp y)::name set)"
-  and     c: "\<exists>(a::name). a\<sharp>f3 \<and> (\<forall>(y::'a::pt_name). a\<sharp>f3 a y)"
-  shows "\<exists>(a''::name). a''\<sharp>(\<lambda>a'. f3 a' (y (pi1@[(a,pi2\<bullet>a')]))) \<and> 
-                       a''\<sharp>(\<lambda>a'. f3 a' (y (pi1@[(a,pi2\<bullet>a')]))) a''" 
-proof -
-  from c obtain a' where d0: "a'\<sharp>f3" and d1: "\<forall>(y::'a::pt_name). a'\<sharp>f3 a' y" by force
-  have "\<exists>(a''::name). a''\<sharp>(f3,a,a',pi1,pi2,y)" 
-    by (rule at_exists_fresh[OF at_name_inst],  simp add: supp_prod fs_name1 a b)
-  then obtain a'' where d2: "a''\<sharp>f3" and d3: "a''\<noteq>a'" and d3b: "a''\<sharp>(f3,a,pi1,pi2,y)" 
-    by (auto simp add: fresh_prod at_fresh[OF at_name_inst])
-  have d3c: "a''\<notin>((supp (f3,a,pi1,pi2,y))::name set)" using d3b by (simp add: fresh_def)
-  have d4: "a''\<sharp>f3 a'' (y (pi1@[(a,pi2\<bullet>a'')]))"
-  proof -
-    have d5: "[(a'',a')]\<bullet>f3 = f3" 
-      by (rule pt_fresh_fresh[OF pt_name_inst, OF at_name_inst, OF d2, OF d0]) 
-    from d1 have "\<forall>(y::'a::pt_name). ([(a'',a')]\<bullet>a')\<sharp>([(a'',a')]\<bullet>(f3 a' y))"
-      by (simp add: pt_fresh_bij[OF pt_name_inst, OF at_name_inst])
-    hence "\<forall>(y::'a::pt_name). a''\<sharp>(f3 a'' ([(a'',a')]\<bullet>y))" using d3 d5 
-      by (simp add: at_calc[OF at_name_inst] pt_fun_app_eq[OF pt_name_inst, OF at_name_inst])
-    hence "a''\<sharp>(f3 a'' ([(a'',a')]\<bullet>((rev [(a'',a')])\<bullet>(y (pi1@[(a,pi2\<bullet>a'')])))))" by force
-    thus ?thesis by (simp only: pt_pi_rev[OF pt_name_inst, OF at_name_inst])
-  qed
-  have d6: "a''\<sharp>(\<lambda>a'. f3 a' (y (pi1@[(a,pi2\<bullet>a')])))"
-  proof -
-    from a b have d7: "finite ((supp (f3,a,pi1,pi2,y))::name set)" by (simp add: supp_prod fs_name1)
-    have e: "((supp (f3,a,pi1,pi2,y))::name set) supports (\<lambda>a'. f3 a' (y (pi1@[(a,pi2\<bullet>a')])))" 
-      by (supports_simp add: perm_append)
-    from e d7 d3c show ?thesis by (rule supports_fresh)
-  qed
-  from d6 d4 show ?thesis by force
-qed
-
-lemma f3_freshness_conditions_simple:
-  fixes f3::"('a::pt_name) f3_ty"
-  and   y ::"name prm \<Rightarrow> 'a::pt_name"
-  and   a ::"name"
-  and   pi::"name prm"
-  assumes a: "finite ((supp f3)::name set)"
-  and     b: "finite ((supp y)::name set)"
-  and     c: "\<exists>(a::name). a\<sharp>f3 \<and> (\<forall>(y::'a::pt_name). a\<sharp>f3 a y)"
-  shows "\<exists>(a''::name). a''\<sharp>(\<lambda>a'. f3 a' (y (pi@[(a,a')]))) \<and> a''\<sharp>(\<lambda>a'. f3 a' (y (pi@[(a,a')]))) a''" 
-proof -
-  from c obtain a' where d0: "a'\<sharp>f3" and d1: "\<forall>(y::'a::pt_name). a'\<sharp>f3 a' y" by force
-  have "\<exists>(a''::name). a''\<sharp>(f3,a,a',pi,y)" 
-    by (rule at_exists_fresh[OF at_name_inst],  simp add: supp_prod fs_name1 a b)
-  then obtain a'' where d2: "a''\<sharp>f3" and d3: "a''\<noteq>a'" and d3b: "a''\<sharp>(f3,a,pi,y)" 
-    by (auto simp add: fresh_prod at_fresh[OF at_name_inst])
-  have d3c: "a''\<notin>((supp (f3,a,pi,y))::name set)" using d3b by (simp add: fresh_def)
-  have d4: "a''\<sharp>f3 a'' (y (pi@[(a,a'')]))"
-  proof -
-    have d5: "[(a'',a')]\<bullet>f3 = f3" 
-      by (rule pt_fresh_fresh[OF pt_name_inst, OF at_name_inst, OF d2, OF d0]) 
-    from d1 have "\<forall>(y::'a::pt_name). ([(a'',a')]\<bullet>a')\<sharp>([(a'',a')]\<bullet>(f3 a' y))"
-      by (simp add: pt_fresh_bij[OF pt_name_inst, OF at_name_inst])
-    hence "\<forall>(y::'a::pt_name). a''\<sharp>(f3 a'' ([(a'',a')]\<bullet>y))" using d3 d5 
-      by (simp add: at_calc[OF at_name_inst] pt_fun_app_eq[OF pt_name_inst, OF at_name_inst])
-    hence "a''\<sharp>(f3 a'' ([(a'',a')]\<bullet>((rev [(a'',a')])\<bullet>(y (pi@[(a,a'')])))))" by force
-    thus ?thesis by (simp only: pt_pi_rev[OF pt_name_inst, OF at_name_inst])
-  qed
-  have d6: "a''\<sharp>(\<lambda>a'. f3 a' (y (pi@[(a,a')])))"
-  proof -
-    from a b have d7: "finite ((supp (f3,a,pi,y))::name set)" by (simp add: supp_prod fs_name1)
-    have "((supp (f3,a,pi,y))::name set) supports (\<lambda>a'. f3 a' (y (pi@[(a,a')])))" 
-      by (supports_simp add: perm_append)
-    with d7 d3c show ?thesis by (simp add: supports_fresh)
-  qed
-  from d6 d4 show ?thesis by force
-qed
-
-lemma f3_fresh_fun_supports:
-  fixes f3::"('a::pt_name) f3_ty"
-  and   a ::"name"
-  and   pi1::"name prm"
-  and   y ::"name prm \<Rightarrow> 'a::pt_name"
-  assumes a: "finite ((supp f3)::name set)"
-  and     b: "finite ((supp y)::name set)"
-  and     c: "\<exists>(a::name). a\<sharp>f3 \<and> (\<forall>(y::'a::pt_name). a\<sharp>f3 a y)"
-  shows "((supp (f3,a,y))::name set) supports (\<lambda>pi. fresh_fun (\<lambda>a'. f3 a' (y (pi@[(a,a')]))))"
-proof (auto simp add: "op supports_def" perm_fun_def expand_fun_eq fresh_def[symmetric])
-  fix b::"name" and c::"name" and pi::"name prm"
-  assume b1: "b\<sharp>(f3,a,y)"
-  and    b2: "c\<sharp>(f3,a,y)"
-  from b1 b2 have b3: "[(b,c)]\<bullet>f3=f3" and t4: "[(b,c)]\<bullet>a=a" and t5: "[(b,c)]\<bullet>y=y"
-    by (simp_all add: pt_fresh_fresh[OF pt_name_inst, OF at_name_inst] fresh_prod)
-  let ?g = "\<lambda>a'. f3 a' (y (([(b,c)]\<bullet>pi)@[(a,a')]))"
-  and ?h = "\<lambda>a'. f3 a' (y (pi@[(a,a')]))"
-  have a0: "finite ((supp (f3,a,[(b,c)]\<bullet>pi,y))::name set)" using a b 
-    by (simp add: supp_prod fs_name1)
-  have a1: "((supp (f3,a,[(b,c)]\<bullet>pi,y))::name set) supports ?g" by (supports_simp add: perm_append)
-  hence a2: "finite ((supp ?g)::name set)" using a0 by (rule supports_finite)
-  have a3: "\<exists>(a''::name). a''\<sharp>?g \<and> a''\<sharp>(?g a'')"
-    by (rule f3_freshness_conditions_simple[OF a, OF b, OF c])
-  have "((supp (f3,a,y))::name set) \<subseteq> (supp (f3,a,[(b,c)]\<bullet>pi,y))" by (force simp add: supp_prod)
-  have a4: "[(b,c)]\<bullet>?g = ?h" using b1 b2
-    by (simp add: fresh_prod, perm_simp add: perm_append)
-  have "[(b,c)]\<bullet>(fresh_fun ?g) = fresh_fun ([(b,c)]\<bullet>?g)" 
-    by (simp add: fresh_fun_equiv[OF pt_name_inst, OF at_name_inst, OF a2, OF a3])
-  also have "\<dots> = fresh_fun ?h" using a4 by simp
-  finally show "[(b,c)]\<bullet>(fresh_fun ?g) = fresh_fun ?h" .
-qed
-
-lemma f3_fresh_fun_supp_finite:
-  fixes f3::"('a::pt_name) f3_ty"
-  and   a ::"name"
-  and   pi1::"name prm"
-  and   y ::"name prm \<Rightarrow> 'a::pt_name"
-  assumes a: "finite ((supp f3)::name set)"
-  and     b: "finite ((supp y)::name set)"
-  and     c: "\<exists>(a::name). a\<sharp>f3 \<and> (\<forall>(y::'a::pt_name). a\<sharp>f3 a y)"
-  shows "finite ((supp (\<lambda>pi. fresh_fun (\<lambda>a'. f3 a' (y (pi@[(a,a')])))))::name set)"
-proof -
-  have "((supp (f3,a,y))::name set) supports (\<lambda>pi. fresh_fun (\<lambda>a'. f3 a' (y (pi@[(a,a')]))))"
-    using a b c by (rule f3_fresh_fun_supports)
-  moreover
-  have "finite ((supp (f3,a,y))::name set)" using a b by (simp add: supp_prod fs_name1) 
-  ultimately show ?thesis by (rule supports_finite)
-qed
-
-types 'a recT  = "'a f1_ty \<Rightarrow> 'a f2_ty \<Rightarrow> 'a f3_ty \<Rightarrow> (lam\<times>(name prm \<Rightarrow> ('a::pt_name))) set"
-
-consts
-  rec :: "('a::pt_name) recT"
-
-inductive "rec f1 f2 f3"
-intros
-r1: "(Var a,\<lambda>pi. f1 (pi\<bullet>a))\<in>rec f1 f2 f3" 
-r2: "\<lbrakk>finite ((supp y1)::name set);(t1,y1)\<in>rec f1 f2 f3; 
-      finite ((supp y2)::name set);(t2,y2)\<in>rec f1 f2 f3\<rbrakk> 
-      \<Longrightarrow> (App t1 t2,\<lambda>pi. f2 (y1 pi) (y2 pi))\<in>rec f1 f2 f3"
-r3: "\<lbrakk>finite ((supp y)::name set);(t,y)\<in>rec f1 f2 f3\<rbrakk> 
-      \<Longrightarrow> (Lam [a].t,\<lambda>pi. fresh_fun (\<lambda>a'. f3 a' (y (pi@[(a,a')]))))\<in>rec f1 f2 f3"
-
-constdefs
-  rfun' :: "'a f1_ty \<Rightarrow> 'a f2_ty \<Rightarrow> 'a f3_ty \<Rightarrow> lam \<Rightarrow> name prm \<Rightarrow> ('a::pt_name)" 
-  "rfun' f1 f2 f3 t \<equiv> (THE y. (t,y)\<in>rec f1 f2 f3)"
-
-  rfun :: "'a f1_ty \<Rightarrow> 'a f2_ty \<Rightarrow> 'a f3_ty \<Rightarrow> lam \<Rightarrow> ('a::pt_name)" 
-  "rfun f1 f2 f3 t \<equiv> rfun' f1 f2 f3 t ([]::name prm)"
-
-lemma rec_prm_eq[rule_format]:
-  fixes f1 ::"('a::pt_name) f1_ty"
-  and   f2 ::"('a::pt_name) f2_ty"
-  and   f3 ::"('a::pt_name) f3_ty"
-  and   t  ::"lam"
-  and   y  ::"name prm \<Rightarrow> ('a::pt_name)"
-  shows "(t,y)\<in>rec f1 f2 f3 \<Longrightarrow> (\<forall>(pi1::name prm) (pi2::name prm). pi1 \<triangleq> pi2 \<longrightarrow> (y pi1 = y pi2))"
-apply(erule rec.induct)
-apply(auto simp add: pt3[OF pt_name_inst])
-apply(rule_tac f="fresh_fun" in arg_cong)
-apply(auto simp add: expand_fun_eq)
-apply(drule_tac x="pi1@[(a,x)]" in spec)
-apply(drule_tac x="pi2@[(a,x)]" in spec)
-apply(force simp add: prm_eq_def pt2[OF pt_name_inst])
-done
-
-(* silly helper lemma *)
-lemma rec_trans: 
-  fixes f1 ::"('a::pt_name) f1_ty"
-  and   f2 ::"('a::pt_name) f2_ty"
-  and   f3 ::"('a::pt_name) f3_ty"
-  and   t  ::"lam"
-  and   y  ::"name prm \<Rightarrow> ('a::pt_name)"
-  assumes a: "(t,y)\<in>rec f1 f2 f3"
-  and     b: "y=y'"
-  shows   "(t,y')\<in>rec f1 f2 f3"
-using a b by simp
-
-lemma rec_prm_equiv:
-  fixes f1 ::"('a::pt_name) f1_ty"
-  and   f2 ::"('a::pt_name) f2_ty"
-  and   f3 ::"('a::pt_name) f3_ty"
-  and   t  ::"lam"
-  and   y  ::"name prm \<Rightarrow> ('a::pt_name)"
-  and   pi ::"name prm"
-  assumes f: "finite ((supp (f1,f2,f3))::name set)"
-  and     c: "\<exists>(a::name). a\<sharp>f3 \<and> (\<forall>(y::'a::pt_name). a\<sharp>f3 a y)"
-  and     a: "(t,y)\<in>rec f1 f2 f3"
-  shows "(pi\<bullet>t,pi\<bullet>y)\<in>rec (pi\<bullet>f1) (pi\<bullet>f2) (pi\<bullet>f3)"
-using a
-proof (induct)
-  case (r1 c)
-  let ?g ="pi\<bullet>(\<lambda>(pi'::name prm). f1 (pi'\<bullet>c))"
-  and ?g'="\<lambda>(pi'::name prm). (pi\<bullet>f1) (pi'\<bullet>(pi\<bullet>c))"
-  have "?g'=?g" 
-  proof (auto simp only: expand_fun_eq perm_fun_def)
-    fix pi'::"name prm"
-    let ?h = "((rev pi)\<bullet>(pi'\<bullet>(pi\<bullet>c)))"
-    and ?h'= "(((rev pi)\<bullet>pi')\<bullet>c)"
-    have "?h' = ((rev pi)\<bullet>pi')\<bullet>((rev pi)\<bullet>(pi\<bullet>c))" 
-      by (simp add: pt_rev_pi[OF pt_name_inst, OF at_name_inst])
-    also have "\<dots> = ?h"
-      by (simp add: pt_perm_compose[OF pt_name_inst, OF at_name_inst,symmetric])
-    finally show "pi\<bullet>(f1 ?h) = pi\<bullet>(f1 ?h')" by simp
-  qed
-  thus ?case by (force intro: rec_trans rec.r1)
-next
-  case (r2 t1 t2 y1 y2)
-  assume a1: "finite ((supp y1)::name set)"
-  and    a2: "finite ((supp y2)::name set)"
-  and    a3: "(pi\<bullet>t1,pi\<bullet>y1) \<in> rec (pi\<bullet>f1) (pi\<bullet>f2) (pi\<bullet>f3)"
-  and    a4: "(pi\<bullet>t2,pi\<bullet>y2) \<in> rec (pi\<bullet>f1) (pi\<bullet>f2) (pi\<bullet>f3)"
-  from a1 a2 have a1': "finite ((supp (pi\<bullet>y1))::name set)" and a2': "finite ((supp (pi\<bullet>y2))::name set)"
-    by (simp_all add: pt_supp_finite_pi[OF pt_name_inst, OF at_name_inst])
-  let ?g ="pi\<bullet>(\<lambda>(pi'::name prm). f2 (y1 pi') (y2 pi'))"
-  and ?g'="\<lambda>(pi'::name prm). (pi\<bullet>f2) ((pi\<bullet>y1) pi') ((pi\<bullet>y2) pi')"
-  have "?g'=?g" by  (simp add: expand_fun_eq perm_fun_def pt_rev_pi[OF pt_name_inst, OF at_name_inst])
-  thus ?case using a1' a2' a3 a4 by (force intro: rec.r2 rec_trans)
-next
-  case (r3 a t y)
-  assume a1: "finite ((supp y)::name set)"
-  and    a2: "(pi\<bullet>t,pi\<bullet>y) \<in> rec (pi\<bullet>f1) (pi\<bullet>f2) (pi\<bullet>f3)"
-  from a1 have a1': "finite ((supp (pi\<bullet>y))::name set)" 
-    by (simp add: pt_supp_finite_pi[OF pt_name_inst, OF at_name_inst])
-  let ?g ="pi\<bullet>(\<lambda>(pi'::name prm). fresh_fun (\<lambda>a'. f3 a' (y (pi'@[(a,a')]))))"
-  and ?g'="(\<lambda>(pi'::name prm). fresh_fun (\<lambda>a'. (pi\<bullet>f3) a' ((pi\<bullet>y) (pi'@[((pi\<bullet>a),a')]))))"
-  have "?g'=?g" 
-  proof (auto simp add: expand_fun_eq perm_fun_def pt_rev_pi[OF pt_name_inst, OF at_name_inst] 
-                        perm_append)
-    fix pi'::"name prm"
-    let ?h  = "\<lambda>a'. pi\<bullet>(f3 ((rev pi)\<bullet>a') (y (((rev pi)\<bullet>pi')@[(a,(rev pi)\<bullet>a')])))"
-    and ?h' = "\<lambda>a'. f3 a' (y (((rev pi)\<bullet>pi')@[(a,a')]))"
-    have fs_f3: "finite ((supp f3)::name set)" using f by (simp add: supp_prod)
-    have fs_h': "finite ((supp ?h')::name set)"
-    proof -
-      have "((supp (f3,a,(rev pi)\<bullet>pi',y))::name set) supports ?h'" 
-	by (supports_simp add: perm_append)
-      moreover
-      have "finite ((supp (f3,a,(rev pi)\<bullet>pi',y))::name set)" using a1 fs_f3 
-	by (simp add: supp_prod fs_name1)
-      ultimately show ?thesis by (rule supports_finite)
-    qed
-    have fcond: "\<exists>(a''::name). a''\<sharp>?h' \<and> a''\<sharp>(?h' a'')"
-      by (rule f3_freshness_conditions_simple[OF fs_f3, OF a1, OF c])
-    have "fresh_fun ?h = fresh_fun (pi\<bullet>?h')"
-      by (simp add: perm_fun_def pt_rev_pi[OF pt_name_inst, OF at_name_inst])
-    also have "\<dots> = pi\<bullet>(fresh_fun ?h')"
-      by (simp add: fresh_fun_equiv[OF pt_name_inst, OF at_name_inst, OF fs_h', OF fcond])
-    finally show "fresh_fun ?h = pi\<bullet>(fresh_fun ?h')" .
-  qed
-  thus ?case using a1' a2 by (force intro: rec.r3 rec_trans)
-qed
-
-
-lemma rec_perm:
-  fixes f1 ::"('a::pt_name) f1_ty"
-  and   f2 ::"('a::pt_name) f2_ty"
-  and   f3 ::"('a::pt_name) f3_ty"
-  and   pi1::"name prm"
-  assumes f: "finite ((supp (f1,f2,f3))::name set)"
-  and     c: "\<exists>(a::name). a\<sharp>f3 \<and> (\<forall>(y::'a::pt_name). a\<sharp>f3 a y)"
-  and     a: "(t,y)\<in>rec f1 f2 f3"
-  shows "(pi1\<bullet>t, \<lambda>pi2. y (pi2@pi1))\<in>rec f1 f2 f3"
-proof -
-  have lem: "\<forall>(y::name prm\<Rightarrow>('a::pt_name))(pi::name prm). 
-             finite ((supp y)::name set) \<longrightarrow> finite ((supp (\<lambda>pi'. y (pi'@pi)))::name set)"
-  proof (intro strip)
-    fix y::"name prm\<Rightarrow>('a::pt_name)" and pi::"name prm"
-    assume  "finite ((supp y)::name set)"
-    hence "finite ((supp (y,pi))::name set)" by (simp add: supp_prod fs_name1)      
-    moreover
-    have  "((supp (y,pi))::name set) supports (\<lambda>pi'. y (pi'@pi))" 
-      by (supports_simp add: perm_append)
-    ultimately show "finite ((supp (\<lambda>pi'. y (pi'@pi)))::name set)" by (simp add: supports_finite)
-  qed
-from a
-show ?thesis
-proof (induct)
-  case (r1 c)
-  show ?case
-    by (auto simp add: pt2[OF pt_name_inst], rule rec.r1)
-next
-  case (r2 t1 t2 y1 y2)
-  thus ?case using lem by (auto intro!: rec.r2) 
-next
-  case (r3 c t y)
-  assume a0: "(t,y)\<in>rec f1 f2 f3"
-  and    a1: "finite ((supp y)::name set)"
-  and    a2: "(pi1\<bullet>t,\<lambda>pi2. y (pi2@pi1))\<in>rec f1 f2 f3"
-  from f have f': "finite ((supp f3)::name set)" by (simp add: supp_prod)
-  show ?case
-  proof(simp)
-    have a3: "finite ((supp (\<lambda>pi2. y (pi2@pi1)))::name set)" using lem a1 by force
-    let ?g' = "\<lambda>(pi::name prm). fresh_fun (\<lambda>a'. f3 a' ((\<lambda>pi2. y (pi2@pi1)) (pi@[(pi1\<bullet>c,a')])))"
-    and ?g  = "\<lambda>(pi::name prm). fresh_fun (\<lambda>a'. f3 a' (y (pi@[(pi1\<bullet>c,a')]@pi1)))"
-    and ?h  = "\<lambda>(pi::name prm). fresh_fun (\<lambda>a'. f3 a' (y (pi@pi1@[(c,a')])))"
-    have eq1: "?g = ?g'" by simp
-    have eq2: "?g'= ?h" 
-    proof (auto simp only: expand_fun_eq)
-      fix pi::"name prm"
-      let ?q  = "\<lambda>a'. f3 a' (y ((pi@[(pi1\<bullet>c,a')])@pi1))"
-      and ?q' = "\<lambda>a'. f3 a' (y (((pi@pi1)@[(c,(rev pi1)\<bullet>a')])))"
-      and ?r  = "\<lambda>a'. f3 a' (y ((pi@pi1)@[(c,a')]))"
-      and ?r' = "\<lambda>a'. f3 a' (y (pi@(pi1@[(c,a')])))"
-      have eq3a: "?r = ?r'" by simp
-      have eq3: "?q = ?q'"
-      proof (auto simp only: expand_fun_eq)
-	fix a'::"name"
-	have "(y ((pi@[(pi1\<bullet>c,a')])@pi1)) =  (y (((pi@pi1)@[(c,(rev pi1)\<bullet>a')])))" 
-	  proof -
-	    have "((pi@[(pi1\<bullet>c,a')])@pi1) \<triangleq> ((pi@pi1)@[(c,(rev pi1)\<bullet>a')])"
-	    by (force simp add: prm_eq_def at_append[OF at_name_inst] 
-                   at_calc[OF at_name_inst] at_bij[OF at_name_inst] 
-                   at_pi_rev[OF at_name_inst] at_rev_pi[OF at_name_inst])
-	    with a0 show ?thesis by (rule rec_prm_eq)
-	  qed
-	thus "f3 a' (y ((pi@[(pi1\<bullet>c,a')])@pi1)) = f3 a' (y (((pi@pi1)@[(c,(rev pi1)\<bullet>a')])))" by simp
-      qed
-      have fs_a: "finite ((supp ?q')::name set)"
-      proof -
-	have "((supp (f3,c,(pi@pi1),(rev pi1),y))::name set) supports ?q'" 
-	  by (supports_simp add: perm_append fresh_list_append fresh_list_rev)
-	moreover
-	have "finite ((supp (f3,c,(pi@pi1),(rev pi1),y))::name set)" using f' a1
-	  by (simp add: supp_prod fs_name1)
-	ultimately show ?thesis by (rule supports_finite)
-      qed
-      have fs_b: "finite ((supp ?r)::name set)"
-      proof -
-	have "((supp (f3,c,(pi@pi1),y))::name set) supports ?r" 
-	  by (supports_simp add: perm_append fresh_list_append)
-	moreover
-	have "finite ((supp (f3,c,(pi@pi1),y))::name set)" using f' a1
-	  by (simp add: supp_prod fs_name1)
-	ultimately show ?thesis by (rule supports_finite)
-      qed
-      have c1: "\<exists>(a''::name). a''\<sharp>?q' \<and> a''\<sharp>(?q' a'')"
-	by (rule f3_freshness_conditions[OF f', OF a1, OF c])
-      have c2: "\<exists>(a''::name). a''\<sharp>?r \<and> a''\<sharp>(?r a'')"
-	by (rule f3_freshness_conditions_simple[OF f', OF a1, OF c])
-      have c3: "\<exists>(d::name). d\<sharp>(?q',?r,(rev pi1))" 
-	by (rule at_exists_fresh[OF at_name_inst], 
-            simp only: finite_Un supp_prod fs_a fs_b fs_name1, simp)
-      then obtain d::"name" where d1: "d\<sharp>?q'" and d2: "d\<sharp>?r" and d3: "d\<sharp>(rev pi1)" 
-	by (auto simp only: fresh_prod)
-      have eq4: "(rev pi1)\<bullet>d = d" using d3 by (simp add: at_prm_fresh[OF at_name_inst])
-      have "fresh_fun ?q = fresh_fun ?q'" using eq3 by simp
-      also have "\<dots> = ?q' d" using fs_a c1 d1 
-	by (simp add: fresh_fun_app[OF pt_name_inst, OF at_name_inst])
-      also have "\<dots> = ?r d" using fs_b c2 d2 eq4
-	by (simp add: fresh_fun_app[OF pt_name_inst, OF at_name_inst])
-      also have "\<dots> = fresh_fun ?r" using fs_b c2 d2 
-	by (simp add: fresh_fun_app[OF pt_name_inst, OF at_name_inst])
-      finally show "fresh_fun ?q = fresh_fun ?r'" by simp
-    qed
-    from a3 a2 have "(Lam [(pi1\<bullet>c)].(pi1\<bullet>t), ?g')\<in>rec f1 f2 f3" by (rule rec.r3)
-    thus "(Lam [(pi1\<bullet>c)].(pi1\<bullet>t), ?h)\<in>rec f1 f2 f3" using eq2 by simp
-  qed
-qed
-qed    
-
-lemma rec_perm_rev:
-  fixes f1::"('a::pt_name) f1_ty"
-  and   f2::"('a::pt_name) f2_ty"
-  and   f3::"('a::pt_name) f3_ty"
-  assumes f: "finite ((supp (f1,f2,f3))::name set)"
-  and     c: "\<exists>(a::name). a\<sharp>f3 \<and> (\<forall>(y::'a::pt_name). a\<sharp>f3 a y)"
-  and     a: "(pi\<bullet>t,y)\<in>rec f1 f2 f3"
-  shows "(t, \<lambda>pi2. y (pi2@(rev pi)))\<in>rec f1 f2 f3"
-proof - 
-  from a have "((rev pi)\<bullet>(pi\<bullet>t),\<lambda>pi2. y (pi2@(rev pi)))\<in>rec f1 f2 f3"
-    by (rule rec_perm[OF f, OF c])
-  thus ?thesis by (simp add: pt_rev_pi[OF pt_name_inst, OF at_name_inst])
-qed
-
-
-lemma rec_unique:
-  fixes f1::"('a::pt_name) f1_ty"
-  and   f2::"('a::pt_name) f2_ty"
-  and   f3::"('a::pt_name) f3_ty"
-  assumes f: "finite ((supp (f1,f2,f3))::name set)"
-  and     c: "\<exists>(a::name). a\<sharp>f3 \<and> (\<forall>(y::'a::pt_name). a\<sharp>f3 a y)"
-  and     a: "(t,y)\<in>rec f1 f2 f3"
-  shows "\<forall>(y'::name prm\<Rightarrow>('a::pt_name))(pi::name prm).
-         (t,y')\<in>rec f1 f2 f3 \<longrightarrow> y pi = y' pi"
-using a
-proof (induct)
-  case (r1 c)
-  show ?case 
-   apply(auto)
-   apply(ind_cases "(Var c, y') \<in> rec f1 f2 f3")
-   apply(simp_all add: lam.distinct lam.inject)
-   done
-next
-  case (r2 t1 t2 y1 y2)
-  thus ?case 
-    apply(clarify)
-    apply(ind_cases "(App t1 t2, y') \<in> rec f1 f2 f3") 
-    apply(simp_all (no_asm_use) only: lam.distinct lam.inject) 
-    apply(clarify)
-    apply(drule_tac x="y1" in spec)
-    apply(drule_tac x="y2" in spec)
-    apply(auto)
-    done
-next
-  case (r3 c t y)
-  assume i1: "finite ((supp y)::name set)"
-  and    i2: "(t,y)\<in>rec f1 f2 f3"
-  and    i3: "\<forall>(y'::name prm\<Rightarrow>('a::pt_name))(pi::name prm).
-              (t,y')\<in>rec f1 f2 f3 \<longrightarrow> y pi = y' pi"
-  from f have f': "finite ((supp f3)::name set)" by (simp add: supp_prod)
-  show ?case 
-  proof (auto)
-    fix y'::"name prm\<Rightarrow>('a::pt_name)" and pi::"name prm"
-    assume i4: "(Lam [c].t, y') \<in> rec f1 f2 f3"
-    from i4 show "fresh_fun (\<lambda>a'. f3 a' (y (pi@[(c,a')]))) = y' pi"
-    proof (cases, simp_all add: lam.distinct lam.inject, auto)
-      fix a::"name" and t'::"lam" and y''::"name prm\<Rightarrow>('a::pt_name)"
-      assume i5: "[c].t = [a].t'"
-      and    i6: "(t',y'')\<in>rec f1 f2 f3"
-      and    i6':"finite ((supp y'')::name set)"
-      let ?g = "\<lambda>a'. f3 a' (y  (pi@[(c,a')]))"
-      and ?h = "\<lambda>a'. f3 a' (y'' (pi@[(a,a')]))"
-      show "fresh_fun ?g = fresh_fun ?h" using i5
-      proof (cases "a=c")
-	case True
-	assume i7: "a=c"
-	with i5 have i8: "t=t'" by (simp add: alpha)
-	show "fresh_fun ?g = fresh_fun ?h" using i3 i6 i7 i8 by simp
-      next
-	case False
-	assume i9: "a\<noteq>c"
-	with i5[symmetric] have i10: "t'=[(a,c)]\<bullet>t" and i11: "a\<sharp>t" by (simp_all add: alpha)
-	have r1: "finite ((supp ?g)::name set)" 
-	proof -
-	  have "((supp (f3,c,pi,y))::name set) supports ?g" 
-	    by (supports_simp add: perm_append)
-	  moreover
-	  have "finite ((supp (f3,c,pi,y))::name set)" using f' i1
-	    by (simp add: supp_prod fs_name1)
-	  ultimately show ?thesis by (rule supports_finite)
-	qed
-	have r2: "finite ((supp ?h)::name set)" 
-	proof -
-	  have "((supp (f3,a,pi,y''))::name set) supports ?h" 
-	    by (supports_simp add: perm_append)
-	  moreover
-	  have "finite ((supp (f3,a,pi,y''))::name set)" using f' i6'
-	    by (simp add: supp_prod fs_name1)
-	  ultimately show ?thesis by (rule supports_finite)
-	qed
-	have c1: "\<exists>(a''::name). a''\<sharp>?g \<and> a''\<sharp>(?g a'')"
-	  by (rule f3_freshness_conditions_simple[OF f', OF i1, OF c])
-	have c2: "\<exists>(a''::name). a''\<sharp>?h \<and> a''\<sharp>(?h a'')"
-	  by (rule f3_freshness_conditions_simple[OF f', OF i6', OF c])
-	have "\<exists>(d::name). d\<sharp>(?g,?h,t,a,c)" 
-	  by (rule at_exists_fresh[OF at_name_inst], 
-              simp only: finite_Un supp_prod r1 r2 fs_name1, simp)
-	then obtain d::"name" 
-	  where f1: "d\<sharp>?g" and f2: "d\<sharp>?h" and f3: "d\<sharp>t" and f4: "d\<noteq>a" and f5: "d\<noteq>c" 
-	  by (force simp add: fresh_prod at_fresh[OF at_name_inst] at_fresh[OF at_name_inst])
-	have g1: "[(a,d)]\<bullet>t = t" 
-	  by (rule pt_fresh_fresh[OF pt_name_inst, OF at_name_inst, OF i11, OF f3]) 
-	from i6 have "(([(a,c)]@[(a,d)])\<bullet>t,y'')\<in>rec f1 f2 f3" using g1 i10 by (simp only: pt_name2)
-	hence "(t, \<lambda>pi2. y'' (pi2@(rev ([(a,c)]@[(a,d)]))))\<in>rec f1 f2 f3"
-	  by (simp only: rec_perm_rev[OF f, OF c])
-	hence g2: "(t, \<lambda>pi2. y'' (pi2@([(a,d)]@[(a,c)])))\<in>rec f1 f2 f3" by simp
-	have "distinct [a,c,d]" using i9 f4 f5 by force
-	hence g3: "(pi@[(c,d)]@[(a,d)]@[(a,c)]) \<triangleq> (pi@[(a,d)])"
-	  by (force simp add: prm_eq_def at_calc[OF at_name_inst] at_append[OF at_name_inst])
-	have "fresh_fun ?g = ?g d" using r1 c1 f1
-	  by (simp add: fresh_fun_app[OF pt_name_inst, OF at_name_inst])
-	also have "\<dots> = f3 d ((\<lambda>pi2. y'' (pi2@([(a,d)]@[(a,c)]))) (pi@[(c,d)]))" using i3 g2 by simp 
-	also have "\<dots> = f3 d (y'' (pi@[(c,d)]@[(a,d)]@[(a,c)]))" by simp
-	also have "\<dots> = f3 d (y'' (pi@[(a,d)]))" using i6 g3 by (simp add: rec_prm_eq)
-	also have "\<dots> = fresh_fun ?h" using r2 c2 f2
-	  by (simp add: fresh_fun_app[OF pt_name_inst, OF at_name_inst])
-	finally show "fresh_fun ?g = fresh_fun ?h" .
-      qed
-    qed
-  qed
-qed
-
-lemma rec_total_aux:
-  fixes f1::"('a::pt_name) f1_ty"
-  and   f2::"('a::pt_name) f2_ty"
-  and   f3::"('a::pt_name) f3_ty"
-  assumes f: "finite ((supp (f1,f2,f3))::name set)"
-  and     c: "\<exists>(a::name). a\<sharp>f3 \<and> (\<forall>(y::'a::pt_name). a\<sharp>f3 a y)"
-  shows "\<exists>(y::name prm\<Rightarrow>('a::pt_name)). ((t,y)\<in>rec f1 f2 f3) \<and> (finite ((supp y)::name set))"
-proof (induct t rule: lam.induct_weak)
-  case (Var c)
-  have a1: "(Var c,\<lambda>(pi::name prm). f1 (pi\<bullet>c))\<in>rec f1 f2 f3" by (rule rec.r1)
-  have a2: "finite ((supp (\<lambda>(pi::name prm). f1 (pi\<bullet>c)))::name set)"
-  proof -
-    have "((supp (f1,c))::name set) supports (\<lambda>(pi::name prm). f1 (pi\<bullet>c))" by (supports_simp)
-    moreover have "finite ((supp (f1,c))::name set)" using f by (simp add: supp_prod fs_name1)
-    ultimately show ?thesis by (rule supports_finite)
-  qed
-  from a1 a2 show ?case by force
-next
-  case (App t1 t2)
-  assume "\<exists>y1. (t1,y1)\<in>rec f1 f2 f3 \<and> finite ((supp y1)::name set)"
-  then obtain y1::"name prm \<Rightarrow> ('a::pt_name)"
-    where a11: "(t1,y1)\<in>rec f1 f2 f3" and a12: "finite ((supp y1)::name set)" by force
-  assume "\<exists>y2. (t2,y2)\<in>rec f1 f2 f3 \<and> finite ((supp y2)::name set)"
-  then obtain y2::"name prm \<Rightarrow> ('a::pt_name)"
-    where a21: "(t2,y2)\<in>rec f1 f2 f3" and a22: "finite ((supp y2)::name set)" by force
-  
-  have a1: "(App t1 t2,\<lambda>(pi::name prm). f2 (y1 pi) (y2 pi))\<in>rec f1 f2 f3"
-    using a12 a11 a22 a21 by (rule rec.r2)
-  have a2: "finite ((supp (\<lambda>(pi::name prm). f2 (y1 pi) (y2 pi)))::name set)"
-  proof -
-    have "((supp (f2,y1,y2))::name set) supports (\<lambda>(pi::name prm). f2 (y1 pi) (y2 pi))" 
-      by (supports_simp)
-    moreover have "finite ((supp (f2,y1,y2))::name set)" using f a21 a22 
-      by (simp add: supp_prod fs_name1)
-    ultimately show ?thesis by (rule supports_finite)
-  qed
-  from a1 a2 show ?case by force
-next
-  case (Lam a t)
-  assume "\<exists>y. (t,y)\<in>rec f1 f2 f3 \<and> finite ((supp y)::name set)"
-  then obtain y::"name prm \<Rightarrow> ('a::pt_name)"
-    where a11: "(t,y)\<in>rec f1 f2 f3" and a12: "finite ((supp y)::name set)" by force
-  from f have f': "finite ((supp f3)::name set)" by (simp add: supp_prod)
-  have a1: "(Lam [a].t,\<lambda>(pi::name prm). fresh_fun (\<lambda>a'. f3 a' (y (pi@[(a,a')]))))\<in>rec f1 f2 f3"
-    using a12 a11 by (rule rec.r3)
-  have a2: "finite ((supp (\<lambda>pi. fresh_fun (\<lambda>a'. f3 a' (y (pi@[(a,a')])))))::name set)" 
-    using f' a12 c by (rule f3_fresh_fun_supp_finite)
-  from a1 a2 show ?case by force
-qed
-
-lemma rec_total:
-  fixes f1::"('a::pt_name) f1_ty"
-  and   f2::"('a::pt_name) f2_ty"
-  and   f3::"('a::pt_name) f3_ty"
-  assumes f: "finite ((supp (f1,f2,f3))::name set)"
-  and     c: "\<exists>(a::name). a\<sharp>f3 \<and> (\<forall>(y::'a::pt_name). a\<sharp>f3 a y)"
-  shows "\<exists>(y::name prm\<Rightarrow>('a::pt_name)). ((t,y)\<in>rec f1 f2 f3)"
-proof -
-  have "\<exists>y. ((t,y)\<in>rec f1 f2 f3) \<and> (finite ((supp y)::name set))"
-    by (rule rec_total_aux[OF f, OF c])
-  thus ?thesis by force
-qed
-
-lemma rec_function:
-  fixes f1::"('a::pt_name) f1_ty"
-  and   f2::"('a::pt_name) f2_ty"
-  and   f3::"('a::pt_name) f3_ty"
-  assumes f: "finite ((supp (f1,f2,f3))::name set)"
-  and     c: "\<exists>(a::name). a\<sharp>f3 \<and> (\<forall>(y::'a::pt_name). a\<sharp>f3 a y)"
-  shows "\<exists>!y. (t,y)\<in>rec f1 f2 f3"
-proof (rule ex_ex1I)
-  case goal1
-  show ?case by (rule rec_total[OF f, OF c])
-next
-  case (goal2 y1 y2)
-  assume a1: "(t,y1)\<in>rec f1 f2 f3" and a2: "(t,y2)\<in>rec f1 f2 f3"
-  hence "\<forall>pi. y1 pi = y2 pi" using rec_unique[OF f, OF c] by force
-  thus ?case by (force simp add: expand_fun_eq) 
-qed
-  
-lemma theI2':
-  assumes a1: "P a" 
-  and     a2: "\<exists>!x. P x" 
-  and     a3: "P a \<Longrightarrow> Q a"
-  shows "Q (THE x. P x)"
-apply(rule theI2)
-apply(rule a1)
-apply(subgoal_tac "\<exists>!x. P x")
-apply(auto intro: a1 simp add: Ex1_def)
-apply(fold Ex1_def)
-apply(rule a2)
-apply(subgoal_tac "x=a")
-apply(simp)
-apply(rule a3)
-apply(assumption)
-apply(subgoal_tac "\<exists>!x. P x")
-apply(auto intro: a1 simp add: Ex1_def)
-apply(fold Ex1_def)
-apply(rule a2)
-done
-
-lemma rfun'_equiv:
-  fixes f1::"('a::pt_name) f1_ty"
-  and   f2::"('a::pt_name) f2_ty"
-  and   f3::"('a::pt_name) f3_ty"
-  and   pi::"name prm"
-  and   t ::"lam"  
-  assumes f: "finite ((supp (f1,f2,f3))::name set)"
-  and     c: "\<exists>(a::name). a\<sharp>f3 \<and> (\<forall>(y::'a::pt_name). a\<sharp>f3 a y)"
-  shows "pi\<bullet>(rfun' f1 f2 f3 t) = rfun' (pi\<bullet>f1) (pi\<bullet>f2) (pi\<bullet>f3) (pi\<bullet>t)"
-apply(auto simp add: rfun'_def)
-apply(subgoal_tac "\<exists>y. (t,y)\<in>rec f1 f2 f3 \<and> finite ((supp y)::name set)")
-apply(auto)
-apply(rule sym)
-apply(rule_tac a="y" in theI2')
-apply(assumption)
-apply(rule rec_function[OF f, OF c])
-apply(rule the1_equality)
-apply(rule rec_function)
-apply(subgoal_tac "finite ((supp (f1,f2,f3))::name set)")
-apply(simp add: supp_prod)
-apply(simp add: pt_supp_finite_pi[OF pt_name_inst, OF at_name_inst])
-apply(rule f)
-apply(subgoal_tac "\<exists>(a::name). a\<sharp>f3 \<and> (\<forall>(y::'a::pt_name). a\<sharp>f3 a y)")
-apply(auto)
-apply(rule_tac x="pi\<bullet>a" in exI)
-apply(auto)
-apply(simp add: pt_fresh_bij[OF pt_name_inst, OF at_name_inst])
-apply(drule_tac x="(rev pi)\<bullet>x" in spec)
-apply(subgoal_tac "(pi\<bullet>f3) (pi\<bullet>a) x  = pi\<bullet>(f3 a ((rev pi)\<bullet>x))")
-apply(simp add: pt_fresh_bij[OF pt_name_inst, OF at_name_inst])
-apply(subgoal_tac "pi\<bullet>(f3 a ((rev pi)\<bullet>x)) = (pi\<bullet>f3) (pi\<bullet>a) (pi\<bullet>((rev pi)\<bullet>x))")
-apply(simp)
-apply(simp add: pt_pi_rev[OF pt_name_inst, OF at_name_inst])
-apply(simp add: pt_fun_app_eq[OF pt_name_inst, OF at_name_inst])
-apply(rule c)
-apply(rule rec_prm_equiv)
-apply(rule f, rule c, assumption)
-apply(rule rec_total_aux)
-apply(rule f)
-apply(rule c)
-done
-
-lemma rfun'_equiv_aux:
-  fixes pi::"name prm"
-  assumes f: "finite ((supp (f1,f2,f3))::name set)"
-  and     c: "\<exists>(a::name). a\<sharp>f3 \<and> (\<forall>(y::'a::pt_name). a\<sharp>f3 a y)"
-  shows "pi\<bullet>(rfun' f1 f2 f3 t pi') = (pi\<bullet>rfun' f1 f2 f3 t) (pi\<bullet>pi')" 
-by (simp add: perm_app)
-
-lemma rfun'_supports:
-  fixes f1::"('a::pt_name) f1_ty"
-  and   f2::"('a::pt_name) f2_ty"
-  and   f3::"('a::pt_name) f3_ty"
-  assumes f: "finite ((supp (f1,f2,f3))::name set)"
-  and     c: "\<exists>(a::name). a\<sharp>f3 \<and> (\<forall>(y::'a::pt_name). a\<sharp>f3 a y)"
-  shows "((supp (f1,f2,f3,t))::name set) supports (rfun' f1 f2 f3 t)"
-proof (auto simp add: "op supports_def" fresh_def[symmetric])
-  fix a::"name" and b::"name"
-  assume a1: "a\<sharp>(f1,f2,f3,t)"
-  and    a2: "b\<sharp>(f1,f2,f3,t)"
-  from a1 a2 have "[(a,b)]\<bullet>f1=f1" and "[(a,b)]\<bullet>f2=f2" and "[(a,b)]\<bullet>f3=f3" and "[(a,b)]\<bullet>t=t"
-    by (simp_all add: pt_fresh_fresh[OF pt_name_inst, OF at_name_inst] fresh_prod)
-  thus "[(a,b)]\<bullet>(rfun' f1 f2 f3 t) = rfun' f1 f2 f3 t"
-    by (simp add: rfun'_equiv[OF f, OF c])
-qed
-
-lemma rfun'_finite_supp:
-  fixes f1::"('a::pt_name) f1_ty"
-  and   f2::"('a::pt_name) f2_ty"
-  and   f3::"('a::pt_name) f3_ty"
-  assumes f: "finite ((supp (f1,f2,f3))::name set)"
-  and     c: "\<exists>(a::name). a\<sharp>f3 \<and> (\<forall>(y::'a::pt_name). a\<sharp>f3 a y)"
-  shows "finite ((supp (rfun' f1 f2 f3 t))::name set)"
-apply(rule supports_finite)
-apply(rule rfun'_supports[OF f, OF c])
-apply(subgoal_tac "finite ((supp (f1,f2,f3))::name set)")
-apply(simp add: supp_prod fs_name1)
-apply(rule f)
-done
-
-lemma rfun'_prm:
-  fixes f1::"('a::pt_name) f1_ty"
-  and   f2::"('a::pt_name) f2_ty"
-  and   f3::"('a::pt_name) f3_ty"
-  and   pi1::"name prm"
-  and   pi2::"name prm"
-  and   t ::"lam"  
-  assumes f: "finite ((supp (f1,f2,f3))::name set)"
-  and     c: "\<exists>(a::name). a\<sharp>f3 \<and> (\<forall>(y::'a::pt_name). a\<sharp>f3 a y)"
-  shows "rfun' f1 f2 f3 (pi1\<bullet>t) pi2 = rfun' f1 f2 f3 t (pi2@pi1)"
-apply(auto simp add: rfun'_def)
-apply(subgoal_tac "\<exists>y. (t,y)\<in>rec f1 f2 f3 \<and> finite ((supp y)::name set)")
-apply(auto)
-apply(rule_tac a="y" in theI2')
-apply(assumption)
-apply(rule rec_function[OF f, OF c])
-apply(rule_tac a="\<lambda>pi2. y (pi2@pi1)" in theI2')
-apply(rule rec_perm)
-apply(rule f, rule c)
-apply(assumption)
-apply(rule rec_function)
-apply(rule f)
-apply(rule c)
-apply(simp)
-apply(rule rec_total_aux)
-apply(rule f)
-apply(rule c)
-done
-
-lemma rfun_Var:
-  fixes f1::"('a::pt_name) f1_ty"
-  and   f2::"('a::pt_name) f2_ty"
-  and   f3::"('a::pt_name) f3_ty"
-  assumes f: "finite ((supp (f1,f2,f3))::name set)"
-  and     c: "\<exists>(a::name). a\<sharp>f3 \<and> (\<forall>(y::'a::pt_name). a\<sharp>f3 a y)"
-  shows "rfun f1 f2 f3 (Var c) = (f1 c)"
-apply(auto simp add: rfun_def rfun'_def)
-apply(subgoal_tac "(THE y. (Var c, y) \<in> rec f1 f2 f3) = (\<lambda>(pi::name prm). f1 (pi\<bullet>c))")(*A*)
-apply(simp)
-apply(rule the1_equality)
-apply(rule rec_function)
-apply(rule f)
-apply(rule c)
-apply(rule rec.r1)
-done
-
-lemma rfun_App:
-  fixes f1::"('a::pt_name) f1_ty"
-  and   f2::"('a::pt_name) f2_ty"
-  and   f3::"('a::pt_name) f3_ty"
-  assumes f: "finite ((supp (f1,f2,f3))::name set)"
-  and     c: "\<exists>(a::name). a\<sharp>f3 \<and> (\<forall>(y::'a::pt_name). a\<sharp>f3 a y)"
-  shows "rfun f1 f2 f3 (App t1 t2) = (f2 (rfun f1 f2 f3 t1) (rfun f1 f2 f3 t2))"
-apply(auto simp add: rfun_def rfun'_def)
-apply(subgoal_tac "(THE y. (App t1 t2, y)\<in>rec f1 f2 f3) = 
-      (\<lambda>(pi::name prm). f2 ((rfun' f1 f2 f3 t1) pi) ((rfun' f1 f2 f3 t2) pi))")(*A*)
-apply(simp add: rfun'_def)
-apply(rule the1_equality)
-apply(rule rec_function[OF f, OF c])
-apply(rule rec.r2)
-apply(rule rfun'_finite_supp[OF f, OF c])
-apply(subgoal_tac "\<exists>y. (t1,y)\<in>rec f1 f2 f3")
-apply(erule exE, simp add: rfun'_def)
-apply(rule_tac a="y" in theI2')
-apply(assumption)
-apply(rule rec_function[OF f, OF c])
-apply(assumption)
-apply(rule rec_total[OF f, OF c])
-apply(rule rfun'_finite_supp[OF f, OF c])
-apply(subgoal_tac "\<exists>y. (t2,y)\<in>rec f1 f2 f3")
-apply(auto simp add: rfun'_def)
-apply(rule_tac a="y" in theI2')
-apply(assumption)
-apply(rule rec_function[OF f, OF c])
-apply(assumption)
-apply(rule rec_total[OF f, OF c])
-done 
-
-lemma rfun_Lam_aux1:
-  fixes f1::"('a::pt_name) f1_ty"
-  and   f2::"('a::pt_name) f2_ty"
-  and   f3::"('a::pt_name) f3_ty"
-  assumes f: "finite ((supp (f1,f2,f3))::name set)"
-  and     c: "\<exists>(a::name). a\<sharp>f3 \<and> (\<forall>(y::'a::pt_name). a\<sharp>f3 a y)"
-  shows "rfun f1 f2 f3 (Lam [a].t) = fresh_fun (\<lambda>a'. f3 a' (rfun' f1 f2 f3 t ([]@[(a,a')])))"
-apply(simp add: rfun_def rfun'_def)
-apply(subgoal_tac "(THE y. (Lam [a].t, y)\<in>rec f1 f2 f3) = 
-        (\<lambda>(pi::name prm). fresh_fun(\<lambda>a'. f3 a' ((rfun' f1 f2 f3 t) (pi@[(a,a')]))))")(*A*)
-apply(simp add: rfun'_def[symmetric])
-apply(rule the1_equality)
-apply(rule rec_function[OF f, OF c])
-apply(rule rec.r3)
-apply(rule rfun'_finite_supp[OF f, OF c])
-apply(subgoal_tac "\<exists>y. (t,y)\<in>rec f1 f2 f3")
-apply(erule exE, simp add: rfun'_def)
-apply(rule_tac a="y" in theI2')
-apply(assumption)
-apply(rule rec_function[OF f, OF c])
-apply(assumption)
-apply(rule rec_total[OF f, OF c])
-done
-
-lemma rfun_Lam_aux2:
-  fixes f1::"('a::pt_name) f1_ty"
-  and   f2::"('a::pt_name) f2_ty"
-  and   f3::"('a::pt_name) f3_ty"
-  assumes f: "finite ((supp (f1,f2,f3))::name set)"
-  and     c: "\<exists>(a::name). a\<sharp>f3 \<and> (\<forall>(y::'a::pt_name). a\<sharp>f3 a y)"
-  and     a: "b\<sharp>(a,t,f1,f2,f3)"
-  shows "rfun f1 f2 f3 (Lam [b].([(a,b)]\<bullet>t)) = f3 b (rfun f1 f2 f3 ([(a,b)]\<bullet>t))"
-proof -
-  from f have f': "finite ((supp f3)::name set)" by (simp add: supp_prod)
-  have eq1: "rfun f1 f2 f3 (Lam [b].([(a,b)]\<bullet>t)) = rfun f1 f2 f3 (Lam [a].t)"
-  proof -
-    have "Lam [a].t = Lam [b].([(a,b)]\<bullet>t)" using a
-      by (force simp add: lam.inject alpha fresh_prod at_fresh[OF at_name_inst]
-             pt_swap_bij[OF pt_name_inst, OF at_name_inst] 
-             pt_fresh_left[OF pt_name_inst, OF at_name_inst] at_calc[OF at_name_inst])
-    thus ?thesis by simp
-  qed
-  let ?g = "(\<lambda>a'. f3 a' (rfun' f1 f2 f3 t ([]@[(a,a')])))"
-  have a0: "((supp (f3,a,([]::name prm),rfun' f1 f2 f3 t))::name set) supports ?g"
-    by (supports_simp add: perm_append rfun'_equiv_aux[OF f, OF c])
-  have a1: "finite ((supp (f3,a,([]::name prm),rfun' f1 f2 f3 t))::name set)"
-    using f' by (simp add: supp_prod fs_name1 rfun'_finite_supp[OF f, OF c])
-  from a0 a1 have a2: "finite ((supp ?g)::name set)"
-    by (rule supports_finite)
-  have c0: "finite ((supp (rfun' f1 f2 f3 t))::name set)"
-    by (rule rfun'_finite_supp[OF f, OF c])
-  have c1: "\<exists>(a''::name). a''\<sharp>?g \<and> a''\<sharp>(?g a'')"
-    by (rule f3_freshness_conditions_simple[OF f', OF c0, OF c])
-  have c2: "b\<sharp>?g"
-  proof -
-    have fs_g: "finite ((supp (f1,f2,f3,t))::name set)" using f
-      by (simp add: supp_prod fs_name1)
-    have "((supp (f1,f2,f3,t))::name set) supports (rfun' f1 f2 f3 t)"
-      by (simp add: rfun'_supports[OF f, OF c])
-    hence c3: "b\<sharp>(rfun' f1 f2 f3 t)" using fs_g 
-    proof(rule supports_fresh, simp add: fresh_def[symmetric])
-      show "b\<sharp>(f1,f2,f3,t)" using a by (simp add: fresh_prod)
-    qed
-    show ?thesis 
-    proof(rule supports_fresh[OF a0, OF a1], simp add: fresh_def[symmetric])
-      show "b\<sharp>(f3,a,([]::name prm),rfun' f1 f2 f3 t)" using a c3
-	by (simp add: fresh_prod fresh_list_nil)
-    qed
-  qed
-  (* main proof *)
-  have "rfun f1 f2 f3 (Lam [b].([(a,b)]\<bullet>t)) = rfun f1 f2 f3 (Lam [a].t)" by (simp add: eq1)
-  also have "\<dots> = fresh_fun ?g" by (rule rfun_Lam_aux1[OF f, OF c])
-  also have "\<dots> = ?g b" using c2
-    by (rule fresh_fun_app[OF pt_name_inst, OF at_name_inst, OF a2, OF c1])
-  also have "\<dots> = f3 b (rfun f1 f2 f3 ([(a,b)]\<bullet>t))"
-    by (simp add: rfun_def rfun'_prm[OF f, OF c])
-  finally show "rfun f1 f2 f3 (Lam [b].([(a,b)]\<bullet>t)) = f3 b (rfun f1 f2 f3 ([(a,b)]\<bullet>t))" .
-qed
-
-
-lemma rfun_Lam:
-  fixes f1::"('a::pt_name) f1_ty"
-  and   f2::"('a::pt_name) f2_ty"
-  and   f3::"('a::pt_name) f3_ty"
-  assumes f: "finite ((supp (f1,f2,f3))::name set)"
-  and     c: "\<exists>(a::name). a\<sharp>f3 \<and> (\<forall>(y::'a::pt_name). a\<sharp>f3 a y)"
-  and     a: "b\<sharp>(f1,f2,f3)"
-  shows "rfun f1 f2 f3 (Lam [b].t) = f3 b (rfun f1 f2 f3 t)"
-proof -
-  have "\<exists>(a::name). a\<sharp>(b,t)"
-    by (rule at_exists_fresh[OF at_name_inst], simp add: supp_prod fs_name1)
-  then obtain a::"name" where a1: "a\<sharp>b" and a2: "a\<sharp>t" by (force simp add: fresh_prod)
-  have "rfun f1 f2 f3 (Lam [b].t) = rfun f1 f2 f3 (Lam [b].(([(a,b)])\<bullet>([(a,b)]\<bullet>t)))"
-    by (simp add: pt_swap_bij[OF pt_name_inst, OF at_name_inst])
-  also have "\<dots> = f3 b (rfun f1 f2 f3 (([(a,b)])\<bullet>([(a,b)]\<bullet>t)))" 
-  proof(rule rfun_Lam_aux2[OF f, OF c])
-    have "b\<sharp>([(a,b)]\<bullet>t)" using a1 a2
-      by (simp add: pt_fresh_left[OF pt_name_inst, OF at_name_inst] at_calc[OF at_name_inst] 
-        at_fresh[OF at_name_inst])
-    thus "b\<sharp>(a,[(a,b)]\<bullet>t,f1,f2,f3)" using a a1 by (force simp add: fresh_prod at_fresh[OF at_name_inst])
-  qed
-  also have "\<dots> = f3 b (rfun f1 f2 f3 t)" by (simp add: pt_swap_bij[OF pt_name_inst, OF at_name_inst])
-  finally show ?thesis .
-qed
-  
-lemma rec_unique:
-  fixes fun::"lam \<Rightarrow> ('a::pt_name)"
-  and   f1::"('a::pt_name) f1_ty"
-  and   f2::"('a::pt_name) f2_ty"
-  and   f3::"('a::pt_name) f3_ty"
-  assumes f: "finite ((supp (f1,f2,f3))::name set)"
-  and     c: "\<exists>(a::name). a\<sharp>f3 \<and> (\<forall>(y::'a::pt_name). a\<sharp>f3 a y)"
-  and     a1: "\<forall>c. fun (Var c) = f1 c" 
-  and     a2: "\<forall>t1 t2. fun (App t1 t2) = f2 (fun t1) (fun t2)" 
-  and     a3: "\<forall>a t. a\<sharp>(f1,f2,f3) \<longrightarrow> fun (Lam [a].t) = f3 a (fun t)"
-  shows "fun t = rfun f1 f2 f3 t"
-apply (rule lam.induct'[of "\<lambda>_. ((supp (f1,f2,f3))::name set)" "\<lambda>_ t. fun t = rfun f1 f2 f3 t"])
-apply(fold fresh_def)
-(* finite support *)
-apply(rule f)
-(* VAR *)
-apply(simp add: a1 rfun_Var[OF f, OF c, symmetric])
-(* APP *)
-apply(simp add: a2 rfun_App[OF f, OF c, symmetric])
-(* LAM *)
-apply(simp add: a3 rfun_Lam[OF f, OF c, symmetric])
-done
-
-lemma rec_function:
-  fixes f1::"('a::pt_name) f1_ty"
-  and   f2::"('a::pt_name) f2_ty"
-  and   f3::"('a::pt_name) f3_ty"
-  assumes f: "finite ((supp (f1,f2,f3))::name set)"
-  and     c: "\<exists>(a::name). a\<sharp>f3 \<and> (\<forall>(y::'a::pt_name). a\<sharp>f3 a y)"
-  shows "(\<exists>!(fun::lam \<Rightarrow> ('a::pt_name)).
-              (\<forall>c.     fun (Var c)     = f1 c) \<and> 
-              (\<forall>t1 t2. fun (App t1 t2) = f2 (fun t1) (fun t2)) \<and> 
-              (\<forall>a t.   a\<sharp>(f1,f2,f3) \<longrightarrow> fun (Lam [a].t) = f3 a (fun t)))"
-apply(rule_tac a="\<lambda>t. rfun f1 f2 f3 t" in ex1I)
-(* existence *)
-apply(simp add: rfun_Var[OF f, OF c])
-apply(simp add: rfun_App[OF f, OF c])
-apply(simp add: rfun_Lam[OF f, OF c])
-(* uniqueness *)
-apply(auto simp add: expand_fun_eq)
-apply(rule rec_unique[OF f, OF c])
-apply(force)+
-done
-
-(* "real" recursion *)
-
-types 'a f1_ty' = "name\<Rightarrow>('a::pt_name)"
-      'a f2_ty' = "lam\<Rightarrow>lam\<Rightarrow>'a\<Rightarrow>'a\<Rightarrow>('a::pt_name)"
-      'a f3_ty' = "lam\<Rightarrow>name\<Rightarrow>'a\<Rightarrow>('a::pt_name)"
-
-constdefs
-  rfun_gen' :: "'a f1_ty' \<Rightarrow> 'a f2_ty' \<Rightarrow> 'a f3_ty' \<Rightarrow> lam \<Rightarrow> (lam\<times>'a::pt_name)" 
-  "rfun_gen' f1 f2 f3 t \<equiv> (rfun 
-                             (\<lambda>(a::name). (Var a,f1 a)) 
-                             (\<lambda>r1 r2. (App (fst r1) (fst r2), f2 (fst r1) (fst r2) (snd r1) (snd r2))) 
-                             (\<lambda>(a::name) r. (Lam [a].(fst r),f3 (fst r) a (snd r)))
-                           t)"
-
-  rfun_gen :: "'a f1_ty' \<Rightarrow> 'a f2_ty' \<Rightarrow> 'a f3_ty' \<Rightarrow> lam \<Rightarrow> 'a::pt_name" 
-  "rfun_gen f1 f2 f3 t \<equiv> snd(rfun_gen' f1 f2 f3 t)"
-
-
-
-lemma f1'_supports:
-  fixes f1::"('a::pt_name) f1_ty'"
-  shows "((supp f1)::name set) supports (\<lambda>(a::name). (Var a,f1 a))"
-  by (supports_simp)
-
-lemma f2'_supports:
-  fixes f2::"('a::pt_name) f2_ty'"
-  shows "((supp f2)::name set) supports 
-                         (\<lambda>r1 r2. (App (fst r1) (fst r2), f2 (fst r1) (fst r2) (snd r1) (snd r2)))"
-  by (supports_simp add: perm_fst perm_snd)  
-
-lemma f3'_supports:
-  fixes f3::"('a::pt_name) f3_ty'"
-  shows "((supp f3)::name set) supports (\<lambda>(a::name) r. (Lam [a].(fst r),f3 (fst r) a (snd r)))"
-by (supports_simp add: perm_fst perm_snd)
-
-lemma fcb': 
-  fixes f3::"('a::pt_name) f3_ty'"
-  assumes f: "finite ((supp (f1,f2,f3))::name set)"
-  and     c: "\<exists>(a::name). a\<sharp>f3 \<and> (\<forall>(y::'a::pt_name) t. a\<sharp>f3 t a y)"
-  shows  "\<exists>a.  a \<sharp> (\<lambda>a r. (Lam [a].fst r, f3 (fst r) a (snd r))) \<and>
-                (\<forall>y.  a \<sharp> (Lam [a].fst y, f3 (fst y) a (snd y)))"
-using c f
-apply(auto)
-apply(rule_tac x="a" in exI)
-apply(auto simp add: abs_fresh fresh_prod)
-apply(rule supports_fresh)
-apply(rule f3'_supports)
-apply(simp add: supp_prod)
-apply(simp add: fresh_def)
-done
-
-lemma fsupp':
-  fixes f1::"('a::pt_name) f1_ty'"
-  and   f2::"('a::pt_name) f2_ty'"
-  and   f3::"('a::pt_name) f3_ty'"
-  assumes f: "finite ((supp (f1,f2,f3))::name set)"
-  shows "finite((supp
-          (\<lambda>a. (Var a, f1 a),
-           \<lambda>r1 r2.
-              (App (fst r1) (fst r2),
-               f2 (fst r1) (fst r2) (snd r1) (snd r2)),
-           \<lambda>a r. (Lam [a].fst r, f3 (fst r) a (snd r))))::name set)"
-using f
-apply(auto simp add: supp_prod)
-apply(rule supports_finite)
-apply(rule f1'_supports)
-apply(assumption)
-apply(rule supports_finite)
-apply(rule f2'_supports)
-apply(assumption)
-apply(rule supports_finite)
-apply(rule f3'_supports)
-apply(assumption)
-done
-
-lemma rfun_gen'_fst:
-  fixes f1::"('a::pt_name) f1_ty'"
-  and   f2::"('a::pt_name) f2_ty'"
-  and   f3::"('a::pt_name) f3_ty'"
-  assumes f: "finite ((supp (f1,f2,f3))::name set)" 
-  and     c: "(\<exists>(a::name). a\<sharp>f3 \<and> (\<forall>(y::'a::pt_name) t. a\<sharp>f3 t a y))"
-  shows "fst (rfun_gen' f1 f2 f3 t) = t"
-apply(rule lam.induct'[of "\<lambda>_. ((supp (f1,f2,f3))::name set)" "\<lambda>_ t. fst (rfun_gen' f1 f2 f3 t) = t"])
-apply(fold fresh_def)
-apply(simp add: f)
-apply(unfold rfun_gen'_def)
-apply(simp only: rfun_Var[OF fsupp'[OF f],OF fcb'[OF f, OF c]])
-apply(simp)
-apply(simp only: rfun_App[OF fsupp'[OF f],OF fcb'[OF f, OF c]])
-apply(simp)
-apply(auto)
-apply(rule trans)
-apply(rule_tac f="fst" in arg_cong)
-apply(rule rfun_Lam[OF fsupp'[OF f],OF fcb'[OF f, OF c]])
-apply(auto simp add: fresh_prod)
-apply(rule supports_fresh)
-apply(rule f1'_supports)
-apply(subgoal_tac "finite ((supp (f1,f2,f3))::name set)")
-apply(simp add: supp_prod)
-apply(rule f)
-apply(simp add: fresh_def)
-apply(rule supports_fresh)
-apply(rule f2'_supports)
-apply(subgoal_tac "finite ((supp (f1,f2,f3))::name set)")
-apply(simp add: supp_prod)
-apply(rule f)
-apply(simp add: fresh_def)
-apply(rule supports_fresh)
-apply(rule f3'_supports)
-apply(subgoal_tac "finite ((supp (f1,f2,f3))::name set)")
-apply(simp add: supp_prod)
-apply(rule f)
-apply(simp add: fresh_def)
-done
-
-lemma rfun_gen'_Var:
-  fixes f1::"('a::pt_name) f1_ty'"
-  and   f2::"('a::pt_name) f2_ty'"
-  and   f3::"('a::pt_name) f3_ty'"
-  assumes f: "finite ((supp (f1,f2,f3))::name set)"
-  and     c: "\<exists>(a::name). a\<sharp>f3 \<and> (\<forall>(y::'a::pt_name) t. a\<sharp>f3 t a y)"
-  shows "rfun_gen' f1 f2 f3 (Var c) = (Var c, f1 c)"
-apply(simp add: rfun_gen'_def)
-apply(simp add: rfun_Var[OF fsupp'[OF f],OF fcb'[OF f, OF c]])
-done
-
-lemma rfun_gen'_App:
-  fixes f1::"('a::pt_name) f1_ty'"
-  and   f2::"('a::pt_name) f2_ty'"
-  and   f3::"('a::pt_name) f3_ty'"
-  assumes f: "finite ((supp (f1,f2,f3))::name set)"
-  and     c: "\<exists>(a::name). a\<sharp>f3 \<and> (\<forall>(y::'a::pt_name) t. a\<sharp>f3 t a y)"
-  shows "rfun_gen' f1 f2 f3 (App t1 t2) = 
-                (App t1 t2, f2 t1 t2 (rfun_gen f1 f2 f3 t1) (rfun_gen f1 f2 f3 t2))"
-apply(simp add: rfun_gen'_def)
-apply(rule trans)
-apply(rule rfun_App[OF fsupp'[OF f],OF fcb'[OF f, OF c]])
-apply(fold rfun_gen'_def)
-apply(simp_all add: rfun_gen'_fst[OF f, OF c])
-apply(simp_all add: rfun_gen_def)
-done
-
-lemma rfun_gen'_Lam:
-  fixes f1::"('a::pt_name) f1_ty'"
-  and   f2::"('a::pt_name) f2_ty'"
-  and   f3::"('a::pt_name) f3_ty'"
-  assumes f: "finite ((supp (f1,f2,f3))::name set)"
-  and     c: "\<exists>(a::name). a\<sharp>f3 \<and> (\<forall>(y::'a::pt_name) t. a\<sharp>f3 t a y)"
-  and     a: "b\<sharp>(f1,f2,f3)"
-  shows "rfun_gen' f1 f2 f3 (Lam [b].t) = (Lam [b].t, f3 t b (rfun_gen f1 f2 f3 t))"
-using a f
-apply(simp add: rfun_gen'_def)
-apply(rule trans)
-apply(rule rfun_Lam[OF fsupp'[OF f],OF fcb'[OF f, OF c]])
-apply(auto simp add: fresh_prod)
-apply(rule supports_fresh)
-apply(rule f1'_supports)
-apply(simp add: supp_prod)
-apply(simp add: fresh_def)
-apply(rule supports_fresh)
-apply(rule f2'_supports)
-apply(simp add: supp_prod)
-apply(simp add: fresh_def)
-apply(rule supports_fresh)
-apply(rule f3'_supports)
-apply(simp add: supp_prod)
-apply(simp add: fresh_def)
-apply(fold rfun_gen'_def)
-apply(simp_all add: rfun_gen'_fst[OF f, OF c])
-apply(simp_all add: rfun_gen_def)
-done
-
-lemma rfun_gen_Var:
-  fixes f1::"('a::pt_name) f1_ty'"
-  and   f2::"('a::pt_name) f2_ty'"
-  and   f3::"('a::pt_name) f3_ty'"
-  assumes f: "finite ((supp (f1,f2,f3))::name set)"
-  and     c: "\<exists>(a::name). a\<sharp>f3 \<and> (\<forall>(y::'a::pt_name) t. a\<sharp>f3 t a y)"
-  shows "rfun_gen f1 f2 f3 (Var c) = f1 c"
-apply(unfold rfun_gen_def)
-apply(simp add: rfun_gen'_Var[OF f, OF c])
-done
-
-lemma rfun_gen_App:
-  fixes f1::"('a::pt_name) f1_ty'"
-  and   f2::"('a::pt_name) f2_ty'"
-  and   f3::"('a::pt_name) f3_ty'"
-  assumes f: "finite ((supp (f1,f2,f3))::name set)"
-  and     c: "\<exists>(a::name). a\<sharp>f3 \<and> (\<forall>(y::'a::pt_name) t. a\<sharp>f3 t a y)"
-  shows "rfun_gen f1 f2 f3 (App t1 t2) = f2 t1 t2 (rfun_gen f1 f2 f3 t1) (rfun_gen f1 f2 f3 t2)"
-apply(unfold rfun_gen_def)
-apply(simp add: rfun_gen'_App[OF f, OF c])
-apply(simp add: rfun_gen_def)
-done
-
-lemma rfun_gen_Lam:
-  fixes f1::"('a::pt_name) f1_ty'"
-  and   f2::"('a::pt_name) f2_ty'"
-  and   f3::"('a::pt_name) f3_ty'"
-  assumes f: "finite ((supp (f1,f2,f3))::name set)"
-  and     c: "\<exists>(a::name). a\<sharp>f3 \<and> (\<forall>(y::'a::pt_name) t. a\<sharp>f3 t a y)"
-  and     a: "b\<sharp>(f1,f2,f3)"
-  shows "rfun_gen f1 f2 f3 (Lam [b].t) = f3 t b (rfun_gen f1 f2 f3 t)"
-using a
-apply(unfold rfun_gen_def)
-apply(simp add: rfun_gen'_Lam[OF f, OF c])
-apply(simp add: rfun_gen_def)
-done
 
 constdefs 
   depth_Var :: "name \<Rightarrow> nat"
@@ -1125,7 +16,7 @@ constdefs
   "depth_Lam \<equiv> \<lambda>(a::name) n. n+1"
 
   depth_lam :: "lam \<Rightarrow> nat"
-  "depth_lam \<equiv> rfun depth_Var depth_App depth_Lam"
+  "depth_lam \<equiv> itfun depth_Var depth_App depth_Lam"
 
 lemma supp_depth_Var:
   shows "((supp depth_Var)::name set)={}"
@@ -1151,18 +42,16 @@ lemma supp_depth_Lam:
   apply(simp add: perm_nat_def)
   done
  
-
 lemma fin_supp_depth:
   shows "finite ((supp (depth_Var,depth_App,depth_Lam))::name set)"
-  using supp_depth_Var supp_depth_Lam supp_depth_App
-by (simp add: supp_prod)
+  by (finite_guess add: depth_Var_def depth_App_def depth_Lam_def perm_nat_def fs_name1)
 
 lemma fresh_depth_Lam:
   shows "\<exists>(a::name). a\<sharp>depth_Lam \<and> (\<forall>n. a\<sharp>depth_Lam a n)"
 apply(rule exI)
 apply(rule conjI)
-apply(simp add: fresh_def supp_depth_Lam)
-apply(auto simp add: depth_Lam_def)
+apply(simp add: fresh_def)
+apply(force simp add: supp_depth_Lam)
 apply(unfold fresh_def)
 apply(simp add: supp_def)
 apply(simp add: perm_nat_def)
@@ -1171,14 +60,14 @@ done
 lemma depth_Var:
   shows "depth_lam (Var c) = 1"
 apply(simp add: depth_lam_def)
-apply(simp add: rfun_Var[OF fin_supp_depth, OF fresh_depth_Lam])
+apply(simp add: itfun_Var[OF fin_supp_depth, OF fresh_depth_Lam])
 apply(simp add: depth_Var_def)
 done
 
 lemma depth_App:
   shows "depth_lam (App t1 t2) = (max (depth_lam t1) (depth_lam t2))+1"
 apply(simp add: depth_lam_def)
-apply(simp add: rfun_App[OF fin_supp_depth, OF fresh_depth_Lam])
+apply(simp add: itfun_App[OF fin_supp_depth, OF fresh_depth_Lam])
 apply(simp add: depth_App_def)
 done
 
@@ -1186,14 +75,12 @@ lemma depth_Lam:
   shows "depth_lam (Lam [a].t) = (depth_lam t)+1"
 apply(simp add: depth_lam_def)
 apply(rule trans)
-apply(rule rfun_Lam[OF fin_supp_depth, OF fresh_depth_Lam])
+apply(rule itfun_Lam[OF fin_supp_depth, OF fresh_depth_Lam])
 apply(simp add: fresh_def supp_prod supp_depth_Var supp_depth_App supp_depth_Lam)
 apply(simp add: depth_Lam_def)
 done
 
-
-(* substitution *)
-
+text {* substitution *}
 constdefs 
   subst_Var :: "name \<Rightarrow>lam \<Rightarrow> name \<Rightarrow> lam"
   "subst_Var b t \<equiv> \<lambda>a. (if a=b then t else (Var a))"
@@ -1205,8 +92,7 @@ constdefs
   "subst_Lam b t \<equiv> \<lambda>a r. Lam [a].r"
 
   subst_lam :: "name \<Rightarrow> lam \<Rightarrow> lam \<Rightarrow> lam"
-  "subst_lam b t \<equiv> rfun (subst_Var b t) (subst_App b t) (subst_Lam b t)"
-
+  "subst_lam b t \<equiv> itfun (subst_Var b t) (subst_App b t) (subst_Lam b t)"
 
 lemma supports_subst_Var:
   shows "((supp (b,t))::name set) supports (subst_Var b t)"
@@ -1218,12 +104,11 @@ done
 
 lemma supports_subst_App:
   shows "((supp (b,t))::name set) supports subst_App b t"
-by (supports_simp add: subst_App_def)
+by  (supports_simp add: subst_App_def)
 
 lemma supports_subst_Lam:
   shows "((supp (b,t))::name set) supports subst_Lam b t"
   by (supports_simp add: subst_Lam_def)
-
 
 lemma fin_supp_subst:
   shows "finite ((supp (subst_Var b t,subst_App b t,subst_Lam b t))::name set)"
@@ -1257,14 +142,14 @@ done
 lemma subst_Var:
   shows "subst_lam b t (Var a) = (if a=b then t else (Var a))"
 apply(simp add: subst_lam_def)
-apply(auto simp add: rfun_Var[OF fin_supp_subst, OF fresh_subst_Lam])
+apply(auto simp add: itfun_Var[OF fin_supp_subst, OF fresh_subst_Lam])
 apply(auto simp add: subst_Var_def)
 done
 
 lemma subst_App:
   shows "subst_lam b t (App t1 t2) = App (subst_lam b t t1) (subst_lam b t t2)"
 apply(simp add: subst_lam_def)
-apply(auto simp add: rfun_App[OF fin_supp_subst, OF fresh_subst_Lam])
+apply(auto simp add: itfun_App[OF fin_supp_subst, OF fresh_subst_Lam])
 apply(auto simp add: subst_App_def)
 done
 
@@ -1274,7 +159,7 @@ lemma subst_Lam:
 using a
 apply(simp add: subst_lam_def)
 apply(subgoal_tac "a\<sharp>(subst_Var b t,subst_App b t,subst_Lam b t)")
-apply(auto simp add: rfun_Lam[OF fin_supp_subst, OF fresh_subst_Lam])
+apply(auto simp add: itfun_Lam[OF fin_supp_subst, OF fresh_subst_Lam])
 apply(simp (no_asm) add: subst_Lam_def)
 apply(auto simp add: fresh_prod)
 apply(rule supports_fresh)
@@ -1292,17 +177,13 @@ lemma subst_Lam':
   assumes a: "a\<noteq>b"
   and     b: "a\<sharp>t"
   shows "subst_lam b t (Lam [a].t1) = Lam [a].(subst_lam b t t1)"
-apply(rule subst_Lam)
-apply(simp add: fresh_prod a b fresh_atm)
-done
+by (simp add: subst_Lam fresh_prod a b fresh_atm)
 
 lemma subst_Lam'':
   assumes a: "a\<sharp>b"
   and     b: "a\<sharp>t"
   shows "subst_lam b t (Lam [a].t1) = Lam [a].(subst_lam b t t1)"
-apply(rule subst_Lam)
-apply(simp add: fresh_prod a b)
-done
+by (simp add: subst_Lam fresh_prod a b)
 
 consts
   subst_syn  :: "lam \<Rightarrow> name \<Rightarrow> lam \<Rightarrow> lam" ("_[_::=_]" [100,100,100] 900)
@@ -1325,15 +206,15 @@ apply(nominal_induct t1 avoiding: b t2 rule: lam.induct)
 apply(auto simp add: perm_bij fresh_prod fresh_atm)
 apply(subgoal_tac "(pi\<bullet>name)\<sharp>(pi\<bullet>b,pi\<bullet>t2)")(*A*)
 apply(simp)
-(*A*) 
-apply(simp add: perm_bij fresh_prod fresh_atm pt_fresh_bij[OF pt_name_inst, OF at_name_inst]) 
+(*A*)
+apply(simp add: pt_fresh_right[OF pt_name_inst, OF at_name_inst], perm_simp add: fresh_prod fresh_atm) 
 done
 
-lemma subst_supp: "supp(t1[a::=t2])\<subseteq>(((supp(t1)-{a})\<union>supp(t2))::name set)"
+lemma subst_supp: 
+  shows "supp(t1[a::=t2]) \<subseteq> (((supp(t1)-{a})\<union>supp(t2))::name set)"
 apply(nominal_induct t1 avoiding: a t2 rule: lam.induct)
 apply(auto simp add: lam.supp supp_atm fresh_prod abs_supp)
-apply(blast)
-apply(blast)
+apply(blast)+
 done
 
 (* parallel substitution *)
@@ -1378,7 +259,7 @@ constdefs
   "psubst_Lam \<theta> \<equiv> \<lambda>a r. Lam [a].r"
 
   psubst_lam :: "(name\<times>lam) list \<Rightarrow> lam \<Rightarrow> lam"
-  "psubst_lam \<theta> \<equiv> rfun (psubst_Var \<theta>) (psubst_App \<theta>) (psubst_Lam \<theta>)"
+  "psubst_lam \<theta> \<equiv> itfun (psubst_Var \<theta>) (psubst_App \<theta>) (psubst_Lam \<theta>)"
 
 lemma supports_psubst_Var:
   shows "((supp \<theta>)::name set) supports (psubst_Var \<theta>)"
@@ -1424,14 +305,14 @@ done
 lemma psubst_Var:
   shows "psubst_lam \<theta> (Var a) = (if a\<in>set (domain \<theta>) then \<theta><a> else (Var a))"
 apply(simp add: psubst_lam_def)
-apply(auto simp add: rfun_Var[OF fin_supp_psubst, OF fresh_psubst_Lam])
+apply(auto simp add: itfun_Var[OF fin_supp_psubst, OF fresh_psubst_Lam])
 apply(auto simp add: psubst_Var_def)
 done
 
 lemma psubst_App:
   shows "psubst_lam \<theta> (App t1 t2) = App (psubst_lam \<theta> t1) (psubst_lam \<theta> t2)"
 apply(simp add: psubst_lam_def)
-apply(auto simp add: rfun_App[OF fin_supp_psubst, OF fresh_psubst_Lam])
+apply(auto simp add: itfun_App[OF fin_supp_psubst, OF fresh_psubst_Lam])
 apply(auto simp add: psubst_App_def)
 done
 
@@ -1441,7 +322,7 @@ lemma psubst_Lam:
 using a
 apply(simp add: psubst_lam_def)
 apply(subgoal_tac "a\<sharp>(psubst_Var \<theta>,psubst_App \<theta>,psubst_Lam \<theta>)")
-apply(auto simp add: rfun_Lam[OF fin_supp_psubst, OF fresh_psubst_Lam])
+apply(auto simp add: itfun_Lam[OF fin_supp_psubst, OF fresh_psubst_Lam])
 apply(simp (no_asm) add: psubst_Lam_def)
 apply(auto simp add: fresh_prod)
 apply(rule supports_fresh)
